Logic/Modal/Basic/Soundness.lean
@@ -10,25 +10,25 @@ open Formula FrameConsequence
 
 variable {α β : Type u}
 
-theorem LogicK.sounds (Γ : Set (Formula α)) (p : Formula α) (f : Frame β) (d : Γ ⊢ᴴ(𝐊) p) : (Γ ⊨ᶠ[f] p) := by
-  induction d <;> try {simp_all [satisfies_imp, satisfies];}
+theorem LogicK.sounds (Γ : Set (Formula α)) (hΓ : Γ = ∅) (p : Formula α) (f : Frame β) (d : Γ ⊢ᴴ(𝐊) p) : (Γ ⊨ᶠ[f] p) := by
+  induction d <;> try {simp_all [satisfies];}
   case wk _ _ _ hΓΔ _ ih =>
-    apply preserveWeakening hΓΔ ih;
+    simp_all only [def_emptyctx];
+    exact ih (by aesop);
   case maxm Γ p ih =>
     let ⟨_, ⟨_, hq⟩⟩ := ih; rw [←hq];
-    apply preserveAxiomK;
+    apply preserve_AxiomK;
   case disj₃ p q r =>
     intro V w;
-    by_cases (w ⊧ˢ[⟨f, V⟩] p) <;> simp_all [satisfies_imp, satisfies];
-  case necessitation _ p _ ih =>
-    exact preserveNecessitation ih;
+    -- TODO: ここで排中律を仮定する必要は本当にあるのだろうか？
+    by_cases (w ⊧ˢ[⟨f, V⟩] p) <;> simp_all [satisfies];
 
 lemma LogicK.weakSounds {p : Formula α} (f : Frame β) (h : ⊢ᴴ(𝐊) p) : (⊧ᶠ[f] p) := by
-  simpa using sounds ∅ p f h;
+  exact (show (⊢ᴴ(𝐊) p) → (⊧ᶠ[f] p) by simpa [Context.box_empty] using sounds (∅) rfl p f;) h;
 
 theorem LogicK.unprovable_bot {f : Frame β} : (⊬ᴴ(𝐊)! (⊥ : Formula α)) := by
   by_contra hC; simp at hC;
-  suffices h : ⊧ᶠ[f] (⊥ : Formula α) by exact frames_bot h;
+  suffices h : ⊧ᶠ[f] (⊥ : Formula α) by exact frames.bot_def h;
   exact weakSounds f hC.some;
 
 end Hilbert
